Redefine compilation based on the ordering

Regex/NFA/Basic.lean
@@ -1,4 +1,4 @@
-import Mathlib.Computability.EpsilonNFA
+import Mathlib.Data.Set.Basic
 
 namespace NFA
 
@@ -10,55 +10,31 @@ inductive Node where
   | split (next₁ next₂ : Nat)
 deriving Repr
 
-def Node.inBounds (n : Node) (nodes : Array Node) : Bool :=
+def Node.charStep (n : Node) (c : Char) : Set Nat :=
   match n with
-  | Node.done | Node.fail => true
-  | Node.epsilon next | Node.char _ next => next < nodes.size
-  | Node.split next₁ next₂ => next₁ < nodes.size && next₂ < nodes.size
+  | Node.char c' next => if c == c' then {next} else ∅
+  | _ => ∅
 
-theorem Node.inBounds.epsilon (h : inBounds (.epsilon next) nodes) : next < nodes.size := by
-  simp [inBounds] at h
-  assumption
+def Node.εStep (n : Node) : Set Nat :=
+  match n with
+  | Node.epsilon next => {next}
+  | Node.split next₁ next₂ => {next₁, next₂}
+  | _ => ∅
 
-theorem Node.inBounds.char (h : inBounds (.char c next) nodes) : next < nodes.size := by
-  simp [inBounds] at h
-  assumption
+/--
+  The NFA consists an array of nodes and a designated start node.
 
-theorem Node.inBounds.splitL (h : inBounds (.split next₁ next₂) nodes) : next₁ < nodes.size := by
-  simp [inBounds] at h
-  exact h.left
-
-theorem Node.inBounds.splitR (h : inBounds (.split next₁ next₂) nodes) : next₂ < nodes.size := by
-  simp [inBounds] at h
-  exact h.right
-
+  The transition relation and accept nodes are embedded in the nodes themselves.
+-/
 structure NFA where
   nodes : Array Node
   start : Fin nodes.size
-  inBounds : ∀ id : Fin nodes.size, nodes[id].inBounds nodes
 deriving Repr
 
-abbrev NodeId (nfa : NFA) := Fin nfa.nodes.size
+def NFA.get (nfa : NFA) (i : Nat) (h : i < nfa.nodes.size) : Node :=
+  nfa.nodes[i]
 
-abbrev SafeNode (nfa : NFA) := { n : Node // n.inBounds nfa.nodes }
-
-def NFA.get (nfa : NFA) (id : NodeId nfa) : SafeNode nfa :=
-  ⟨nfa.nodes[id], nfa.inBounds id⟩
-
-def NFA.step (nfa : NFA) (id : NodeId nfa) (c : Option Char) : Set (NodeId nfa) :=
-  match nfa.get id, c with
-  | ⟨.char c' next, prop⟩, some c => if c = c' then {⟨next, Node.inBounds.char prop⟩} else ∅
-  | ⟨.epsilon next, prop⟩, none => {⟨next, Node.inBounds.epsilon prop⟩}
-  | ⟨.split next₁ next₂, prop⟩, none =>
-    {⟨next₁, Node.inBounds.splitL prop⟩, ⟨next₂, Node.inBounds.splitR prop⟩}
-  | _, _ => ∅
-
-def NFA.accept (nfa : NFA) : Set (NodeId nfa) := { id : NodeId nfa | (nfa.get id).val = .done }
-
-def NFA.toMathlibεNFA (nfa : NFA) : εNFA Char (NodeId nfa) :=
-  ⟨nfa.step, {nfa.start}, nfa.accept⟩
-
-def NFA.accepts (nfa : NFA) (cs : List Char) :=
-  (nfa.toMathlibεNFA).accepts cs
+instance : GetElem NFA Nat Node (fun nfa i => i < nfa.nodes.size) where
+  getElem := NFA.get
 
 end NFA
