Regex/NFA/Compile.lean
@@ -1,166 +1,103 @@
+import Regex.Lemmas
 import Regex.Regex
 import Regex.NFA.Basic
-
-import Mathlib.Tactic.Common
+import Regex.NFA.Order
 
 namespace NFA
 
-def addNode (nodes : Array Node) (node : Node) :
-  (nodes' : { nodes' : Array Node // nodes.size < nodes'.size}) × Fin nodes'.val.size :=
-  have lt_size : nodes.size < (nodes.push node).size := by
+def NFA.addNode (nfa : NFA) (node : Node) :
+  { nfa' : NFA // nfa ≤ nfa' } :=
+  have isLt : nfa.nodes.size < (nfa.nodes.push node).size := by
     simp [Array.size_push]
-  have isLt : nodes.size < (nodes.push node).size := by
-    simp [Array.size_push]
-  ⟨⟨nodes.push node, lt_size⟩, ⟨nodes.size, isLt⟩⟩
+  let start := nfa.nodes.size
+  let nfa' : NFA := ⟨nfa.nodes.push node, ⟨start, isLt⟩⟩
 
-theorem addNode.get_lt {nodes : Array Node} {node : Node} {i : Nat} (h : i < nodes.size) :
-  (addNode nodes node).1.val[i]'(Nat.lt_trans h (addNode nodes node).1.property) = nodes[i] := by
-  simp [addNode]
-  apply Array.get_push_lt
+  have property : nfa ≤ nfa' := by
+    intro i h
+    have h' : i < nfa'.nodes.size := Nat.lt_trans h isLt
+    have eq : nfa'[i] = nfa[i] := by
+      apply Array.get_push_lt
+    exact ⟨h', Node.le_of_eq eq.symm⟩
 
-@[simp]
-theorem addNode.get_eq {nodes : Array Node} {node : Node} :
-  (addNode nodes node).1.val[(addNode nodes node).2.val] = node := by
-  show (addNode nodes node).1.val[(addNode nodes node).2.val] = node
-  simp [addNode]
+  ⟨nfa', property⟩
 
-/--
-  Thompson construction algorithm for converting the given regex to NFA.
--/
-def compileRaw (r : Regex) :
-  (nodes : Array Node) × Fin nodes.size :=
-  let result := loop #[.done] 0 r
-  ⟨result.1.val, result.2⟩
+def compile (r : Regex) : NFA :=
+  let result := loop r 0 ⟨#[.done], ⟨0, Nat.zero_lt_succ _⟩⟩
+  result.val
 where
   /--
     The main loop of the compilation.
 
-    It compiles the given regex into the given `nodes`. The compiled nodes transition to `next`
-    if and only if the input matches. It returns the new `nodes` and the corresponding ID for the
-    given regex in the array.
+    It compiles the given regex into nodes that transitions to `next` on match.
+    Returned NFA contains the compiled nodes at the end and starts at the node
+    corresponding to the given regex.
   -/
-  loop (nodes : Array Node) (next : Nat) :
-    Regex → (nodes' : { nodes' : Array Node // nodes.size < nodes'.size}) × Fin nodes'.val.size
-  | .empty => addNode nodes .fail
-  | .epsilon => addNode nodes (.epsilon next)
-  | .char c => addNode nodes (.char c next)
+  loop (r : Regex) (next : Nat) (nfa : NFA) : { nfa' // nfa ≤ nfa' } := match r with
+  | .empty => nfa.addNode .fail
+  | .epsilon => nfa.addNode (.epsilon next)
+  | .char c => nfa.addNode (.char c next)
   | .alternate r₁ r₂ =>
-    let ⟨nodes₁, start₁⟩ := loop nodes next r₁
-    let ⟨nodes₂, start₂⟩ := loop nodes₁ next r₂
-    let ⟨nodes', start⟩ := addNode nodes₂ (.split start₁ start₂)
+    -- TODO: it feels better to compile r₂ first to align with concat
+    let nfa₁ := loop r₁ next nfa
+    let start₁ := nfa₁.val.start
+    let nfa₂ := loop r₂ next nfa₁
+    let start₂ := nfa₂.val.start
+    let nfa' := nfa₂.val.addNode (.split start₁ start₂)
 
-    have property : nodes.size < nodes'.val.size :=
-      calc nodes.size
-        _ < nodes₁.val.size := nodes₁.property
-        _ < nodes₂.val.size := nodes₂.property
-        _ < nodes'.val.size := nodes'.property
+    have property : nfa ≤ nfa' :=
+      calc nfa
+        _ ≤ nfa₁.val := nfa₁.property
+        _ ≤ nfa₂.val := nfa₂.property
+        _ ≤ nfa' := nfa'.property
 
-    ⟨⟨nodes', property⟩, start⟩
+    ⟨nfa', property⟩
   | .concat r₁ r₂ =>
-    let ⟨nodes₂, start₂⟩ := loop nodes next r₂
-    let ⟨nodes₁, start₁⟩ := loop nodes₂ start₂ r₁
+    let nfa₂ := loop r₂ next nfa
+    let nfa₁ := loop r₁ next nfa₂
 
-    have property : nodes.size < nodes₁.val.size :=
-      calc nodes.size
-        _ < nodes₂.val.size := nodes₂.property
-        _ < nodes₁.val.size := nodes₁.property
+    have property : nfa ≤ nfa₁ :=
+      calc nfa
+        _ ≤ nfa₂.val := nfa₂.property
+        _ ≤ nfa₁.val := nfa₁.property
 
-    ⟨⟨nodes₁, property⟩, start₁⟩
+    ⟨nfa₁, property⟩
   | .star r =>
-    -- We need to generate a placeholder node first. We use `done` for it to save an allocation.
+    -- We need to generate a placeholder node first. We use `done` for it because variants
+    -- without data are represented as a boxed integer so there is no allocation.
     -- TODO: check generated code
-    let ⟨nodes', start⟩ := addNode nodes .done
-    let ⟨nodes'', target⟩ := loop nodes' start r
+    let nfa' := nfa.addNode .done
+    let start := nfa'.val.start
+    let nfa'' := loop r start nfa'
 
-    have property : nodes.size < nodes''.val.size :=
-      calc nodes.size
-        _ < nodes'.val.size := nodes'.property
-        _ < nodes''.val.size := nodes''.property
-    have isLt : start.val < nodes''.val.size :=
-      calc start.val
-        _ < nodes'.val.size := start.isLt
-        _ < nodes''.val.size := nodes''.property
+    have property : nfa ≤ nfa'' :=
+      calc nfa
+        _ ≤ nfa'.val := nfa'.property
+        _ ≤ nfa''.val := nfa''.property
+    have isLt : start.val < nfa''.val.nodes.size :=
+      Nat.lt_of_lt_of_le nfa'.val.start.isLt (NFA.le_size_of_le nfa''.property)
 
     -- Patch the placeholder node
-    let nodes''' := nodes''.val.set ⟨start.val, isLt⟩ (.split target next)
+    let target := nfa''.val.start
+    let nodes''' := nfa''.val.nodes.set ⟨start.val, isLt⟩ (.split target next)
 
-    have eq_size : nodes'''.size = nodes''.val.size := by simp
-    have isLt : start.val < nodes'''.size := by
-      rw [eq_size]
-      exact isLt
+    have eq_size : nodes'''.size = nfa''.val.nodes.size := by simp
+    have isLt' : start.val < nodes'''.size := eq_size ▸ isLt
+    let nfa''' := ⟨nodes''', ⟨start.val, isLt'⟩⟩
 
-    ⟨⟨nodes''', eq_size ▸ property⟩, ⟨start.val, isLt⟩⟩
+    have property' : nfa ≤ nfa''' := by
+      intro i h
 
-def compileRaw.loop.get_lt {i : Nat} (h : i < nodes.size) :
-  (loop nodes next r).1.val[i]'(Nat.lt_trans h (loop nodes next r).1.property) = nodes[i] := by
-  -- have isLt := Nat.lt_trans h (loop nodes next r).1.property
-  induction r generalizing nodes next with
-  | empty | epsilon | char c => simp [loop]; apply addNode.get_lt
-  | alternate r₁ r₂ ih₁ ih₂ =>
-    let result₁ := loop nodes next r₁
-    let result₂ := loop result₁.1 next r₂
-    let result := addNode result₂.1 (.split result₁.2 result₂.2)
+      have le_size : nfa.nodes.size ≤ nfa''.val.nodes.size := NFA.le_size_of_le property
+      have h₂ : i < nodes'''.size := Nat.lt_of_lt_of_le h (eq_size ▸ le_size)
+      exists h₂
 
-    have isLt₁ : i < result₁.1.val.size := Nat.lt_trans h result₁.1.property
-    have isLt₂ : i < result₂.1.val.size := Nat.lt_trans isLt₁ result₂.1.property
-    have isLt : i < result.1.val.size := Nat.lt_trans isLt₂ result.1.property
+      have eq : nfa'''[i] = nfa''.val[i]'(Nat.lt_of_lt_of_le h le_size) := by
+        apply Array.get_set_ne
+        exact (Nat.ne_of_gt h)
+      rw [eq]
+      exact (property i _).2
 
-    show result.1.val[i] = nodes[i]
-
-    calc result.1.val[i]
-      _ = result₂.1.val[i] := addNode.get_lt isLt₂
-      _ = result₁.1.val[i] := ih₂ isLt₁
-      _ = nodes[i] := ih₁ h
-  | concat r₁ r₂ ih₁ ih₂ =>
-    let result₂ := loop nodes next r₂
-    let result₁ := loop result₂.1 result₂.2 r₁
-
-    have isLt₂ : i < result₂.1.val.size := Nat.lt_trans h result₂.1.property
-    have isLt₁ : i < result₁.1.val.size := Nat.lt_trans isLt₂ result₁.1.property
-
-    show result₁.1.val[i] = nodes[i]
-
-    calc result₁.1.val[i]
-      _ = result₂.1.val[i] := ih₁ isLt₂
-      _ = nodes[i] := ih₂ h
-  | star r ih =>
-    let result := addNode nodes .done
-    let result' := loop result.1 result.2 r
-
-    have property : nodes.size < result'.1.val.size :=
-      calc nodes.size
-        _ < result.1.val.size := result.1.property
-        _ < result'.1.val.size := result'.1.property
-    have startIsLt : result.2.val < result'.1.val.size :=
-      calc result.2.val
-        _ < result.1.val.size := result.2.isLt
-        _ < result'.1.val.size := result'.1.property
-
-    let nodes' := result'.1.val.set ⟨result.2.val, startIsLt⟩ (.split result'.2 next)
-
-    have eq_size : nodes'.size = result'.1.val.size := by simp
-
-    have isLt : i < result.1.val.size := Nat.lt_trans h result.1.property
-    have isLt' : i < result'.1.val.size := Nat.lt_trans isLt result'.1.property
-    have isLt'' : i < nodes'.size := eq_size ▸ Nat.lt_trans h startIsLt
-
-    show nodes'[i] = nodes[i]
-
-    calc nodes'[i]
-      _ = result'.1.val[i] := by
-        have eq : nodes.size = result.2.val := rfl
-        rw [Array.get_set_ne]
-        exact Nat.ne_of_gt (eq ▸ h)
-      _ = result.1.val[i] := ih isLt
-      _ = nodes[i] := addNode.get_lt h
-
-def compile (r : Regex) : NFA :=
-  let result := compileRaw r
-  let nodes := result.1
-  let start := result.2
-
-  -- TODO: inBoundsはNatを受け取った方が証明が楽そう。nodesの内容を見ないで良いため
-  ⟨nodes, start, sorry⟩
+    ⟨nfa''', property'⟩
 
 #eval compile (Regex.star (Regex.char 'a'))
 #eval compile (Regex.alternate (Regex.char 'a') (Regex.star (Regex.concat (Regex.char 'a') (Regex.char 'b'))))
